Use modules in Termination

ExistentialRules/ChaseSequence/Termination/ConstantMappings/StrictConstantMapping.lean
@@ -1,10 +1,14 @@
-import ExistentialRules.ChaseSequence.Termination.ConstantMappings.Basic
+module
+
+public import ExistentialRules.ChaseSequence.Termination.ConstantMappings.Basic
 
 /-!
 # Strict Constant Mappings
 
 A `StrictConstantMapping` is an even more confined version of a `ConstantMapping` where constants are really just mapped to (other) constants and not arbitrary `GroundTerm`s.
 -/
+
+public section
 
 /-- The `StrictConstantMapping` is simply defined as a `TermMapping`. -/
 abbrev StrictConstantMapping (sig : Signature) [DecidableEq sig.P] [DecidableEq sig.C] [DecidableEq sig.V] := TermMapping sig.C sig.C
@@ -14,15 +18,17 @@ namespace StrictConstantMapping
 variable {sig : Signature} [DecidableEq sig.P] [DecidableEq sig.C] [DecidableEq sig.V]
 
 /-- A `StrictConstantMapping` can be transformed to a `ConstantMapping` in the obvious way. -/
-def toConstantMapping (g : StrictConstantMapping sig) : ConstantMapping sig := GroundTerm.const ∘ g
+abbrev toConstantMapping (g : StrictConstantMapping sig) : ConstantMapping sig := GroundTerm.const ∘ g
 
 /-- We lift `StrictConstantMapping`s to `VarOrConst` in the obvious way. -/
+@[expose]
 def apply_var_or_const (g : StrictConstantMapping sig) : TermMapping (VarOrConst sig) (VarOrConst sig)
 | .var v => .var v
 | .const c => .const (g c)
 
 /-- Applying a `StrictConstantMapping` to a `VarOrConst` does not influence the result of `VarOrConst.filterVars`. -/
-theorem apply_var_or_const_filterVars_eq (g : StrictConstantMapping sig) (vocs : List (VarOrConst sig)) : VarOrConst.filterVars (vocs.map g.apply_var_or_const) = VarOrConst.filterVars vocs := by
+theorem apply_var_or_const_filterVars_eq (g : StrictConstantMapping sig) (vocs : List (VarOrConst sig)) :
+    VarOrConst.filterVars (vocs.map g.apply_var_or_const) = VarOrConst.filterVars vocs := by
   induction vocs with
   | nil => simp
   | cons hd tl ih =>
@@ -32,7 +38,8 @@ theorem apply_var_or_const_filterVars_eq (g : StrictConstantMapping sig) (vocs :
     )
 
 /-- Mapping over the leaves of a `PreGroundTerm` is the same as calling the `FiniteTree.mapLeaves` with the `toConstantMapping` version of the `StrictConstantMapping`. -/
-theorem map_leaves_eq_leaves_mapLeaves (g : StrictConstantMapping sig) (t : FiniteTree (SkolemFS sig) sig.C) : t.leaves.map g = (t.mapLeaves (fun c => (g.toConstantMapping c).val)).leaves := by
+theorem map_leaves_eq_leaves_mapLeaves (g : StrictConstantMapping sig) (t : FiniteTree (SkolemFS sig) sig.C) :
+    t.leaves.map g = (t.mapLeaves (fun c => (g.toConstantMapping c).val)).leaves := by
   induction t with
   | leaf c => simp [FiniteTree.leaves, FiniteTree.mapLeaves, toConstantMapping, GroundTerm.const]
   | inner func ts ih =>
@@ -61,7 +68,8 @@ abbrev apply_function_free_conj (g : StrictConstantMapping sig) : FunctionFreeCo
   TermMapping.apply_generalized_atom_list g.apply_var_or_const
 
 /-- Applying a `StrictConstantMapping` to a `FunctionFreeConjunction` does not change the variables. -/
-theorem apply_function_free_conj_vars_eq (g : StrictConstantMapping sig) (conj : FunctionFreeConjunction sig) : (g.apply_function_free_conj conj).vars = conj.vars := by
+theorem apply_function_free_conj_vars_eq (g : StrictConstantMapping sig) (conj : FunctionFreeConjunction sig) :
+    (g.apply_function_free_conj conj).vars = conj.vars := by
   unfold apply_function_free_conj
   unfold TermMapping.apply_generalized_atom_list
   unfold FunctionFreeConjunction.vars
