ExistentialRules/ChaseSequence/Termination/ConstantMappings/Basic.lean
@@ -1,6 +1,6 @@
-import BasicLeanDatastructures.GetFreshInhabitant
-import ExistentialRules.ChaseSequence.Termination.RenameConstantsApart
-import ExistentialRules.Triggers.Basic
+module
+
+public import ExistentialRules.Triggers.Basic
 
 /-!
 # Constant Mappings
@@ -9,6 +9,8 @@ A `ConstantMapping` is a `TermMapping` from constants to `GroundTerm`s.
 This is very similar to a GroundSubstitution only that it maps constants instead of variables
 -/
 
+public section
+
 abbrev ConstantMapping (sig : Signature) [DecidableEq sig.P] [DecidableEq sig.C] [DecidableEq sig.V] := TermMapping sig.C (GroundTerm sig)
 
 namespace ConstantMapping
@@ -16,13 +18,14 @@ namespace ConstantMapping
 variable {sig : Signature} [DecidableEq sig.P] [DecidableEq sig.C] [DecidableEq sig.V]
 
 /-- The id `ConstantMapping` is the `GroundTerm.const` constructor. -/
-def id : ConstantMapping sig := GroundTerm.const
+abbrev id : ConstantMapping sig := GroundTerm.const
 
 /-- We apply a `ConstantMapping` to a `PreGroundTerm` by applying it to all leaves. -/
 abbrev apply_pre_ground_term (g : ConstantMapping sig) : TermMapping (PreGroundTerm sig) (PreGroundTerm sig) :=
   FiniteTree.mapLeaves (fun c => (g c).val)
 
 /-- Applying the `ConstantMapping.id` on a `PreGroundTerm` yields the same term. -/
+@[simp, grind =]
 theorem apply_pre_ground_term_id (t : FiniteTree (SkolemFS sig) sig.C) : id.apply_pre_ground_term t = t := by
   induction t with
   | leaf c => simp only [apply_pre_ground_term, FiniteTree.mapLeaves]; rfl
@@ -57,7 +60,8 @@ theorem apply_pre_ground_term_arity_ok (g : ConstantMapping sig) (t : FiniteTree
         simp
 
 /-- Mapping the same term using two `ConstantMapping`s yields the same term if the mappings agree on all leaves of the term. -/
-theorem apply_pre_ground_term_congr_left (g g2 : ConstantMapping sig) (t : PreGroundTerm sig) : (∀ c ∈ t.leaves, g c = g2 c) -> g.apply_pre_ground_term t = g2.apply_pre_ground_term t := by
+theorem apply_pre_ground_term_congr_left (g g2 : ConstantMapping sig) (t : PreGroundTerm sig) :
+    (∀ c ∈ t.leaves, g c = g2 c) -> g.apply_pre_ground_term t = g2.apply_pre_ground_term t := by
   intro h
   unfold ConstantMapping.apply_pre_ground_term
   apply FiniteTree.mapLeaves_eq_of_map_leaves_eq
@@ -67,22 +71,27 @@ theorem apply_pre_ground_term_congr_left (g g2 : ConstantMapping sig) (t : PreGr
   rw [h]
 
 /-- If the `ConstantMapping` is the id on the leaves of a term, applying the mapping to the term is also the id. -/
-theorem apply_pre_ground_term_eq_self_of_id_on_constants (g : ConstantMapping sig) (t : PreGroundTerm sig) (id_on_constants : ∀ c ∈ t.leaves, g c = .const c) : g.apply_pre_ground_term t = t := by
+theorem apply_pre_ground_term_eq_self_of_id_on_constants
+    (g : ConstantMapping sig) (t : PreGroundTerm sig) (id_on_constants : ∀ c ∈ t.leaves, g c = .const c) :
+    g.apply_pre_ground_term t = t := by
   unfold ConstantMapping.apply_pre_ground_term
   conv => right; rw [← apply_pre_ground_term_id t]
   apply apply_pre_ground_term_congr_left
   exact id_on_constants
 
 /-- We lift `ConstantMapping`s to `GroundTerm`s in the obvious way. -/
+@[expose]
 def apply_ground_term (g : ConstantMapping sig) : TermMapping (GroundTerm sig) (GroundTerm sig) :=
   fun t => ⟨g.apply_pre_ground_term t.val, g.apply_pre_ground_term_arity_ok t.val t.property⟩
 
 /-- Applying a `ConstantMapping` to a `GroundTerm.const` is the same as directly applying the mapping to the underlying constant. -/
+@[simp, grind =]
 theorem apply_ground_term_constant (g : ConstantMapping sig) : ∀ c, g.apply_ground_term (.const c) = g c := by
   intro c
   simp [apply_ground_term, apply_pre_ground_term, FiniteTree.mapLeaves, GroundTerm.const]
 
 /-- Applyign a `ConstantMapping` to a `GroundTerm.func` is the same as applying the mapping to all child terms. -/
+@[simp, grind =]
 theorem apply_ground_term_func (g : ConstantMapping sig) :
     ∀ func ts arity_ok, g.apply_ground_term (.func func ts arity_ok) = .func func (ts.map g.apply_ground_term) (by rw [List.length_map]; exact arity_ok) := by
   intro func ts arity_ok
@@ -113,13 +122,12 @@ theorem apply_ground_term_swap_apply_skolem_term (g : ConstantMapping sig) (subs
     simp only [apply_pre_ground_term, FiniteTree.mapLeaves]
     simp only [Subtype.mk.injEq, FiniteTree.inner.injEq, true_and]
     unfold List.unattach
-    rw [List.map_map]
-    rw [List.map_map]
-    rw [List.map_map]
+    simp only [List.map_map]
     rfl
 
 /-- Mapping the same term using two `ConstantMapping`s yields the same term if the mappings agree on all constants of the term. -/
-theorem apply_ground_term_congr_left (g g2 : ConstantMapping sig) (t : GroundTerm sig) : (∀ c ∈ t.constants, g c = g2 c) -> g.apply_ground_term t = g2.apply_ground_term t := by
+theorem apply_ground_term_congr_left (g g2 : ConstantMapping sig) (t : GroundTerm sig) :
+    (∀ c ∈ t.constants, g c = g2 c) -> g.apply_ground_term t = g2.apply_ground_term t := by
   intro h
   unfold ConstantMapping.apply_ground_term
   rw [Subtype.mk.injEq]
@@ -127,7 +135,9 @@ theorem apply_ground_term_congr_left (g g2 : ConstantMapping sig) (t : GroundTer
   exact h
 
 /-- If the `ConstantMapping` is the id on the constants of a term, applying the mapping to the term is also the id. -/
-theorem apply_ground_term_eq_self_of_id_on_constants (g : ConstantMapping sig) (t : GroundTerm sig) (id_on_constants : ∀ c ∈ t.constants, g c = .const c) : g.apply_ground_term t = t := by
+theorem apply_ground_term_eq_self_of_id_on_constants
+    (g : ConstantMapping sig) (t : GroundTerm sig) (id_on_constants : ∀ c ∈ t.constants, g c = .const c) :
+    g.apply_ground_term t = t := by
   unfold ConstantMapping.apply_ground_term
   rw [Subtype.mk.injEq]
   apply apply_pre_ground_term_eq_self_of_id_on_constants
@@ -138,32 +148,26 @@ abbrev apply_fact (g : ConstantMapping sig) : Fact sig -> Fact sig := TermMappin
 
 /-- Applying a `ConstantMapping` to a fact can be seens as applying a `GroundTermMapping` to the fact. -/
 theorem apply_fact_eq_groundTermMapping_applyFact (g : ConstantMapping sig) (f : Fact sig) :
-    g.apply_fact f = GroundTermMapping.applyFact g.apply_ground_term f := by
-  simp [apply_fact, GroundTermMapping.applyFact]
+  g.apply_fact f = GroundTermMapping.applyFact g.apply_ground_term f := by rfl
 
 /-- Consider a `ConstantMapping`, a `PreTrigger`, and a `FunctionFreeAtom`. If the constant mapping if the id on all constants in the atom, then applying the mapping after the trigger is the same a applying a trigger where the constant mapping is composed with the original substitution. -/
-theorem apply_fact_swap_apply_to_function_free_atom (g : ConstantMapping sig) (trg : PreTrigger sig) (a : FunctionFreeAtom sig) (h : ∀ d ∈ a.constants, g d = GroundTerm.const d) : ∀ i, g.apply_fact (trg.apply_to_function_free_atom i a) = PreTrigger.apply_to_function_free_atom { rule := trg.rule, subs := g.apply_ground_term ∘ trg.subs } i a := by
+theorem apply_fact_swap_apply_to_function_free_atom (g : ConstantMapping sig) (trg : PreTrigger sig) (a : FunctionFreeAtom sig)
+    (h : ∀ d ∈ a.constants, g d = GroundTerm.const d) :
+    ∀ i, g.apply_fact (trg.apply_to_function_free_atom i a) =
+      PreTrigger.apply_to_function_free_atom { rule := trg.rule, subs := g.apply_ground_term ∘ trg.subs } i a := by
   intro i
   unfold PreTrigger.apply_to_function_free_atom
   unfold ConstantMapping.apply_fact
-  unfold PreTrigger.apply_to_var_or_const
   rw [← TermMapping.apply_generalized_atom_compose']
   apply TermMapping.apply_generalized_atom_congr_left
   intro voc voc_mem
   simp only [Function.comp_apply]
   cases voc with
+  | const d => simpa using h d (by simpa using voc_mem)
   | var v =>
-    rw [ConstantMapping.apply_ground_term_swap_apply_skolem_term]
-    . rfl
-    . intro c contra
-      simp only [PreTrigger.skolemize_var_or_const, VarOrConst.skolemize] at contra
-      split at contra <;> contradiction
-  | const d =>
-    simp only [PreTrigger.skolemize_var_or_const, VarOrConst.skolemize, GroundSubstitution.apply_skolem_term]
-    rw [g.apply_ground_term_constant]
-    apply h
-    apply VarOrConst.mem_filterConsts_of_const
-    exact voc_mem
+    cases Decidable.em (v ∈ trg.rule.frontier) with
+    | inl v_mem => simp [v_mem]
+    | inr v_mem => simp [v_mem, PreTrigger.functional_term_for_var]
 
 /-- Mapping the same fact using two `ConstantMapping`s yields the same fact if the mappings agree on all constants of the fact. -/
 theorem apply_fact_congr_left (g g2 : ConstantMapping sig) (f : Fact sig) : (∀ c ∈ f.constants, g c = g2 c) -> g.apply_fact f = g2.apply_fact f := by
