ExistentialRules/ChaseSequence/Termination/ConstantMappings/InterplayWithBacktracking/BacktrackingUnderConstantMappingSubsetOfComposingWithSubs/GroundTerm.lean
@@ -1,10 +1,14 @@
-import ExistentialRules.ChaseSequence.Termination.ConstantMappings.InterplayWithBacktracking.BacktrackingUnderConstantMappingSubsetOfComposingWithSubs.PreGroundTerm
+module
+
+public import ExistentialRules.ChaseSequence.Termination.ConstantMappings.InterplayWithBacktracking.BacktrackingUnderConstantMappingSubsetOfComposingWithSubs.PreGroundTerm
 
 /-!
 # Interaction of Backtrackings and Strict Constant Mappings on GroundTerm
 
 We merely lift `PreGroundTerm.backtrackFacts_under_constant_mapping_subset_of_composing_with_subs` to `GroundTerm` here.
 -/
+
+public section
 
 variable {sig : Signature} [DecidableEq sig.C] [DecidableEq sig.V] [DecidableEq sig.P]
 
